First imperative pair memory

scratch/Memory_Heap.thy
@@ -1,18 +1,19 @@
 theory Memory_Heap
-  imports State_Heap
+  imports State_Heap Memory
 begin
+
+instance array :: (heap) heap ..
 
 context
   fixes size :: nat
-    and to_index :: "('k :: heap) \<Rightarrow> nat"
-  assumes injective: "\<forall> a b. to_index a = to_index b \<and> to_index b < size \<longrightarrow> a = b"
+    and to_index :: "('k2 :: heap) \<Rightarrow> nat"
 begin
 
 definition
-  "mem_empty = (Array.new size (None :: ('a :: heap) option))"
+  "mem_empty = (Array.new size (None :: ('v :: heap) option))"
 
 context
-  fixes mem :: "('a :: heap) option array"
+  fixes mem :: "('v :: heap) option array"
 begin
 
 definition
@@ -30,7 +31,10 @@ definition
 definition
   "P heap = (Array.length heap mem = size)"
 
-lemma mem_heap_corect: "heap_correct P mem_update mem_lookup"
+context assumes injective: "\<forall> a b. to_index a = to_index b \<and> to_index b < size \<longrightarrow> a = b"
+begin
+
+lemma mem_heap_correct: "heap_correct P mem_update mem_lookup"
   apply standard
   subgoal lookup_inv
     unfolding State_Heap.lift_p_def P_def mem_lookup_def by (simp add: Let_def execute_simps)
@@ -47,8 +51,663 @@ lemma mem_heap_corect: "heap_correct P mem_update mem_lookup"
     done
   done
 
+end (* Injectivity *)
+
 end (* Fixed array *)
 
+context
+  fixes key1 :: "'k \<Rightarrow> ('k1 :: heap)" and key2 :: "'k \<Rightarrow> 'k2"
+    and m_ref1 m_ref2 :: "('v :: heap) option array ref"
+    and k_ref1 k_ref2 :: "('k1 :: heap) ref"
+begin
+
+text \<open>We assume that look-ups happen on the older row, so this is biased towards the second entry.\<close>
+definition
+  "lookup_pair k = (
+    let k' = key1 k in
+      (
+      !k_ref2 \<bind> (\<lambda> k2.
+      if k' = k2 then
+        !m_ref2 \<bind> (\<lambda> m2. mem_lookup m2 (key2 k))
+      else
+        !k_ref1 \<bind> (\<lambda> k1.
+        if k' = k1 then
+          !m_ref1 \<bind> (\<lambda> m1. mem_lookup m1 (key2 k))
+        else
+          return None))
+      )
+      )
+   "
+
+text \<open>We assume that updates happen on the newer row, so this is biased towards the first entry.\<close>
+definition
+  "update_pair k v = (
+    let k' = key1 k in
+      (
+      Heap_Monad.bind (!k_ref1) (\<lambda> k1.
+      if k' = k1 then
+        Heap_Monad.bind (!m_ref1) (\<lambda> m. mem_update m (key2 k) v)
+      else
+        Heap_Monad.bind (!k_ref2) (\<lambda> k2.
+        if k' = k2 then
+          Heap_Monad.bind (!m_ref2) (\<lambda> m. mem_update m (key2 k) v)
+        else
+          Heap_Monad.bind mem_empty (\<lambda> m.
+            Heap_Monad.bind (!m_ref1) (\<lambda> m1.
+              k_ref2 := k1 \<then> k_ref1 := k' \<then> m_ref2 := m1 \<then> m_ref1 := m
+            )
+          )
+        )
+      )
+    )
+   )
+   "
+
+definition
+  "inv_pair heap = (
+    let
+      k1 = Ref.get heap k_ref1;
+      k2 = Ref.get heap k_ref2;
+      m1 = Ref.get heap m_ref1;
+      m2 = Ref.get heap m_ref2
+    in
+    (\<forall> k \<in> dom (heap_mem_defs.map_of_heap (mem_lookup m1) heap). \<exists> k'. key1 k' = k1 \<and> key2 k' = k) \<and>
+    (\<forall> k \<in> dom (heap_mem_defs.map_of_heap (mem_lookup m2) heap). \<exists> k'. key1 k' = k2 \<and> key2 k' = k) \<and>
+    k1 \<noteq> k2 \<and> P TYPE('v) m1 heap \<and> P TYPE('v) m2 heap
+  )"
+
+definition
+  "inv_pair_weak heap = (
+    let
+      m1 = Ref.get heap m_ref1;
+      m2 = Ref.get heap m_ref2
+    in P TYPE('v) m1 heap \<and> P TYPE('v) m2 heap
+      \<and> Array.length heap m1 = size \<and> Array.length heap m2 = size
+      \<and> Ref.present heap k_ref1 \<and> Ref.present heap k_ref2
+      \<and> Ref.present heap m_ref1 \<and> Ref.present heap m_ref2
+      \<and> Array.present heap m1 \<and> Array.present heap m2
+      \<and> m1 =!!= m2
+  )"
+
+lemma inv_pair_P_D1: "P TYPE('v) (Ref.get heap m_ref1) heap" if "inv_pair heap"
+  using that unfolding inv_pair_def by (auto simp: Let_def)
+
+lemma inv_pair_P_D2: "P TYPE('v) (Ref.get heap m_ref2) heap" if "inv_pair heap"
+  using that unfolding inv_pair_def by (auto simp: Let_def)
+
+lemma inv_pair_lengthD1:
+  "Array.length heap (Ref.get heap m_ref1) = size" if "inv_pair_weak heap"
+  using that unfolding inv_pair_weak_def by (auto simp: Let_def)
+
+lemma inv_pair_lengthD2:
+  "Array.length heap (Ref.get heap m_ref2) = size" if "inv_pair_weak heap"
+  using that unfolding inv_pair_weak_def by (auto simp: Let_def)
+
+lemma inv_pair_presentD:
+  "Array.present heap (Ref.get heap m_ref1)" "Array.present heap (Ref.get heap m_ref2)"
+  if "inv_pair_weak heap"
+  using that unfolding inv_pair_weak_def by (auto simp: Let_def)
+
+lemma inv_pair_presentD2:
+  "Ref.present heap m_ref1" "Ref.present heap m_ref2"
+  "Ref.present heap k_ref1" "Ref.present heap k_ref2"
+  if "inv_pair_weak heap"
+  using that unfolding inv_pair_weak_def by (auto simp: Let_def)
+
+lemma inv_pair_not_eqD:
+  "Ref.get heap m_ref1 =!!= Ref.get heap m_ref2" if "inv_pair_weak heap"
+  using that unfolding inv_pair_weak_def by (auto simp: Let_def)
+
+definition "lookup1 k \<equiv> state_of (!m_ref1 \<bind> (\<lambda> m. mem_lookup m k))"
+
+definition "lookup2 k \<equiv> state_of (!m_ref2 \<bind> (\<lambda> m. mem_lookup m k))"
+
+definition "update1 k v \<equiv> state_of (!m_ref1 \<bind> (\<lambda> m. mem_update m k v))"
+
+definition "update2 k v \<equiv> state_of (!m_ref2 \<bind> (\<lambda> m. mem_update m k v))"
+
+definition "move12 k \<equiv>
+  state_of (Heap_Monad.bind (!k_ref1) (\<lambda> k1.
+    Heap_Monad.bind mem_empty (\<lambda> m. Heap_Monad.bind (!m_ref1) (\<lambda> m1.
+      k_ref2 := k1 \<then> k_ref1 := k \<then> m_ref2 := m1 \<then> m_ref1 := m))))"
+
+definition "get_k1 \<equiv> state_of (!k_ref1)"
+
+definition "get_k2 \<equiv> state_of (!k_ref2)"
+
+lemma runState_state_of[simp]:
+  "runState (state_of p) m = the (execute p m)"
+  unfolding state_of_def by simp
+
+context assumes injective: "\<forall> a b. to_index a = to_index b \<and> to_index b < size \<longrightarrow> a = b"
+begin
+
+interpretation m1: heap_correct
+  "P TYPE('v) (Ref.get heap m_ref1)"
+  "mem_update (Ref.get heap m_ref1)"
+  "mem_lookup (Ref.get heap m_ref1)"
+  by (rule mem_heap_correct[OF injective])
+
+interpretation m2: heap_correct
+  "P TYPE('v) (Ref.get heap m_ref2)"
+  "mem_update (Ref.get heap m_ref2)"
+  "mem_lookup (Ref.get heap m_ref2)"
+  by (rule mem_heap_correct[OF injective])
+
+context
+  assumes disjoint[simp]:
+    "m_ref1 =!= m_ref2" "m_ref1 =!= k_ref1" "m_ref1 =!= k_ref2"
+    "m_ref2 =!= k_ref1" "m_ref2 =!= k_ref2"
+    "k_ref1 =!= k_ref2"
+begin
+
+lemmas [simp] = disjoint[THEN noteq_sym]
+
+lemma [simp]:
+  "Array.get (snd (Array.alloc xs heap)) a = Array.get heap a" if "Array.present heap a"
+  using that unfolding Array.alloc_def Array.present_def
+  apply (simp add: Let_def)
+  apply (subst Array.get_set_neq)
+  subgoal
+    by (simp add: Array.noteq_def)
+  subgoal
+    unfolding Array.get_def by simp
+  done
+
+lemma [simp]:
+  "Ref.get (snd (Array.alloc xs heap)) r = Ref.get heap r" if "Ref.present heap r"
+  using that unfolding Array.alloc_def Ref.present_def
+  by (simp add: Let_def Ref.get_def Array.set_def)
+
+lemma alloc_present:
+  "Array.present (snd (Array.alloc xs heap)) a" if "Array.present heap a"
+  using that unfolding Array.present_def Array.alloc_def by (simp add: Let_def Array.set_def)
+
+lemma alloc_present':
+  "Ref.present (snd (Array.alloc xs heap)) r" if "Ref.present heap r"
+  using that unfolding Ref.present_def Array.alloc_def by (simp add: Let_def Array.set_def)
+
+lemma length_get_upd[simp]:
+  "length (Array.get (Array.update a i x heap) r) = length (Array.get heap r)"
+  unfolding Array.get_def Array.update_def Array.set_def by simp
+
+interpretation pair: pair_mem lookup1 lookup2 update1 update2 move12 get_k1 get_k2 inv_pair_weak
+  apply standard
+  subgoal
+    by (simp add: execute_simps get_k1_def)
+  subgoal
+    by (simp add: execute_simps get_k2_def)
+  subgoal
+    by (auto simp:
+      move12_def mem_empty_def mem_defs.map_of_def map_le_def lookup1_def mem_lookup_def
+      execute_bind_success[OF success_newI] execute_simps Let_def Array.get_alloc length_def
+    )
+  subgoal for m k1 x m'
+    apply (frule inv_pair_lengthD1)
+    apply (auto simp:
+      move12_def mem_empty_def mem_defs.map_of_def map_le_def lookup1_def lookup2_def mem_lookup_def
+      execute_bind_success[OF success_newI] execute_simps Let_def Array.get_alloc length_def
+      simp: inv_pair_presentD inv_pair_presentD2
+    )
+    done
+  subgoal
+    by (auto simp:
+      move12_def mem_empty_def mem_defs.map_of_def map_le_def lookup1_def lookup2_def get_k1_def mem_lookup_def
+      execute_bind_success[OF success_newI] execute_simps Let_def Array.get_alloc length_def
+      simp: inv_pair_presentD inv_pair_presentD2
+    )
+  subgoal
+    by (auto simp:
+      move12_def mem_empty_def mem_defs.map_of_def map_le_def lookup1_def lookup2_def get_k1_def get_k2_def mem_lookup_def
+      execute_bind_success[OF success_newI] execute_simps Let_def Array.get_alloc length_def
+      simp: inv_pair_presentD inv_pair_presentD2
+    )
+  subgoal
+    apply (rule lift_pI)
+    unfolding inv_pair_weak_def Memory_Heap.P_def
+    apply (auto simp:
+      move12_def mem_empty_def mem_defs.map_of_def map_le_def lookup1_def lookup2_def get_k1_def get_k2_def mem_lookup_def
+      execute_bind_success[OF success_newI] execute_simps Let_def Array.get_alloc length_def
+      simp: inv_pair_presentD inv_pair_presentD2 
+      intro: alloc_present alloc_present'
+      elim: present_alloc_noteq[THEN Array.noteq_sym]
+    )
+    done
+  subgoal
+    apply (rule lift_pI)
+    unfolding inv_pair_weak_def Memory_Heap.P_def
+    apply (auto simp:
+      move12_def mem_empty_def mem_defs.map_of_def map_le_def lookup1_def lookup2_def get_k1_def get_k2_def mem_lookup_def
+      execute_bind_success[OF success_newI] execute_simps Let_def Array.get_alloc length_def
+      simp: inv_pair_presentD inv_pair_presentD2 
+      intro: alloc_present alloc_present'
+      split: if_split_asm
+    )
+    done
+  subgoal
+    apply (rule lift_pI)
+    unfolding inv_pair_weak_def Memory_Heap.P_def
+    apply (auto simp:
+      move12_def mem_empty_def mem_defs.map_of_def map_le_def lookup1_def lookup2_def get_k1_def get_k2_def mem_lookup_def
+      execute_bind_success[OF success_newI] execute_simps Let_def Array.get_alloc length_def
+      simp: inv_pair_presentD inv_pair_presentD2 
+      intro: alloc_present alloc_present'
+      split: if_split_asm
+    )
+    done
+  subgoal
+    apply (rule lift_pI)
+    unfolding inv_pair_weak_def Memory_Heap.P_def
+    apply (auto simp:
+      move12_def mem_empty_def mem_defs.map_of_def map_le_def update1_def lookup1_def lookup2_def get_k1_def get_k2_def mem_update_def mem_lookup_def
+      execute_bind_success[OF success_newI] execute_simps Let_def Array.get_alloc length_def
+      simp: inv_pair_presentD inv_pair_presentD2 
+      intro: alloc_present alloc_present'
+      split: if_split_asm
+    )
+    done
+  subgoal
+    apply (rule lift_pI)
+    unfolding inv_pair_weak_def Memory_Heap.P_def
+    apply (auto simp:
+      move12_def mem_empty_def mem_defs.map_of_def map_le_def update1_def update2_def lookup1_def lookup2_def get_k1_def get_k2_def mem_update_def mem_lookup_def
+      execute_bind_success[OF success_newI] execute_simps Let_def Array.get_alloc length_def
+      simp: inv_pair_presentD inv_pair_presentD2 
+      intro: alloc_present alloc_present'
+      split: if_split_asm
+    )
+    done
+  subgoal
+    apply (frule inv_pair_lengthD1)
+    apply (auto simp:
+      move12_def mem_empty_def mem_defs.map_of_def map_le_def update1_def update2_def lookup1_def lookup2_def get_k1_def get_k2_def mem_update_def mem_lookup_def
+      execute_bind_success[OF success_newI] execute_simps Let_def Array.get_alloc length_def
+      simp: inv_pair_presentD inv_pair_presentD2 
+      intro: alloc_present alloc_present'
+      split: if_split_asm
+    )
+    done
+  subgoal
+    apply (frule inv_pair_lengthD1)
+    apply (auto simp:
+      move12_def mem_empty_def mem_defs.map_of_def map_le_def update1_def update2_def lookup1_def lookup2_def get_k1_def get_k2_def mem_update_def mem_lookup_def
+      execute_bind_success[OF success_newI] execute_simps Let_def Array.get_alloc length_def
+      simp: inv_pair_presentD inv_pair_presentD2 
+      intro: alloc_present alloc_present'
+      split: if_split_asm
+    )
+    done
+  subgoal
+    apply (frule inv_pair_lengthD2)
+    apply (auto simp:
+      move12_def mem_empty_def mem_defs.map_of_def map_le_def update1_def update2_def lookup1_def lookup2_def get_k1_def get_k2_def mem_update_def mem_lookup_def
+      execute_bind_success[OF success_newI] execute_simps Let_def Array.get_alloc length_def
+      simp: inv_pair_presentD inv_pair_presentD2 
+      intro: alloc_present alloc_present'
+      split: if_split_asm
+    )
+    done
+   subgoal
+    apply (frule inv_pair_lengthD2)
+    apply (auto simp:
+      move12_def mem_empty_def mem_defs.map_of_def map_le_def update1_def update2_def lookup1_def lookup2_def get_k1_def get_k2_def mem_update_def mem_lookup_def
+      execute_bind_success[OF success_newI] execute_simps Let_def Array.get_alloc length_def
+      simp: inv_pair_presentD inv_pair_presentD2 
+      intro: alloc_present alloc_present'
+      split: if_split_asm
+    )
+     done
+   subgoal
+    apply (frule inv_pair_lengthD1)
+    apply (auto simp:
+      move12_def mem_empty_def mem_defs.map_of_def map_le_def update1_def update2_def lookup1_def lookup2_def get_k1_def get_k2_def mem_update_def mem_lookup_def
+      execute_bind_success[OF success_newI] execute_simps Let_def Array.get_alloc length_def
+      simp: inv_pair_presentD inv_pair_presentD2 
+      intro: alloc_present alloc_present'
+      split: if_split_asm
+    )
+     done
+  subgoal
+    apply (frule inv_pair_lengthD1)
+    apply (auto simp:
+      move12_def mem_empty_def mem_defs.map_of_def map_le_def update1_def update2_def lookup1_def lookup2_def get_k1_def get_k2_def mem_update_def mem_lookup_def
+      execute_bind_success[OF success_newI] execute_simps Let_def Array.get_alloc length_def
+      simp: inv_pair_presentD inv_pair_presentD2 
+      intro: alloc_present alloc_present'
+      split: if_split_asm
+    )
+    done
+  subgoal
+    apply (frule inv_pair_lengthD2)
+    apply (auto simp:
+      move12_def mem_empty_def mem_defs.map_of_def map_le_def update1_def update2_def lookup1_def lookup2_def get_k1_def get_k2_def mem_update_def mem_lookup_def
+      execute_bind_success[OF success_newI] execute_simps Let_def Array.get_alloc length_def
+      simp: inv_pair_presentD inv_pair_presentD2 
+      intro: alloc_present alloc_present'
+      split: if_split_asm
+    )
+    done
+  subgoal
+    apply (frule inv_pair_lengthD2)
+    apply (auto simp:
+      move12_def mem_empty_def mem_defs.map_of_def map_le_def update1_def update2_def lookup1_def lookup2_def get_k1_def get_k2_def mem_update_def mem_lookup_def
+      execute_bind_success[OF success_newI] execute_simps Let_def Array.get_alloc length_def
+      simp: inv_pair_presentD inv_pair_presentD2 
+      intro: alloc_present alloc_present'
+      split: if_split_asm
+    )
+    done
+  subgoal
+    apply (frule inv_pair_lengthD1)
+    apply (auto simp:
+      move12_def mem_empty_def mem_defs.map_of_def map_le_def update1_def update2_def lookup1_def lookup2_def get_k1_def get_k2_def mem_update_def mem_lookup_def
+      execute_bind_success[OF success_newI] execute_simps Let_def Array.get_alloc length_def
+      simp: inv_pair_presentD inv_pair_presentD2 
+      intro: alloc_present alloc_present'
+      split: if_split_asm
+    )
+    done
+  subgoal
+    apply (frule inv_pair_lengthD1)
+    apply (auto simp:
+      move12_def mem_empty_def mem_defs.map_of_def map_le_def update1_def update2_def lookup1_def lookup2_def get_k1_def get_k2_def mem_update_def mem_lookup_def
+      execute_bind_success[OF success_newI] execute_simps Let_def Array.get_alloc length_def
+      simp: inv_pair_presentD inv_pair_presentD2 
+      intro: alloc_present alloc_present'
+      split: if_split_asm
+    )
+    done
+  subgoal
+    apply (frule inv_pair_lengthD2)
+    apply (auto simp:
+      move12_def mem_empty_def mem_defs.map_of_def map_le_def update1_def update2_def lookup1_def lookup2_def get_k1_def get_k2_def mem_update_def mem_lookup_def
+      execute_bind_success[OF success_newI] execute_simps Let_def Array.get_alloc length_def
+      simp: inv_pair_presentD inv_pair_presentD2 
+      intro: alloc_present alloc_present'
+      split: if_split_asm
+    )
+    done
+  subgoal
+    apply (frule inv_pair_lengthD2)
+    apply (auto simp:
+      move12_def mem_empty_def mem_defs.map_of_def map_le_def update1_def update2_def lookup1_def lookup2_def get_k1_def get_k2_def mem_update_def mem_lookup_def
+      execute_bind_success[OF success_newI] execute_simps Let_def Array.get_alloc length_def
+      simp: inv_pair_presentD inv_pair_presentD2 
+      intro: alloc_present alloc_present'
+      split: if_split_asm
+    )
+    done
+  subgoal
+    apply (frule inv_pair_lengthD1)
+    apply (frule inv_pair_lengthD2)
+    apply (auto simp:
+      move12_def mem_empty_def mem_defs.map_of_def map_le_def update1_def update2_def Memory_Heap.lookup1_def lookup2_def get_k1_def get_k2_def mem_update_def Memory_Heap.mem_lookup_def
+      execute_bind_success[OF success_newI] execute_simps Let_def Array.get_alloc length_def
+      simp: inv_pair_presentD inv_pair_presentD2 
+      intro: alloc_present alloc_present'
+      split: if_split_asm
+    )
+    using injective
+    apply (subst (asm) nth_list_update_neq)
+    by auto
+ subgoal
+    apply (frule inv_pair_lengthD1)
+    apply (frule inv_pair_lengthD2)
+    apply (auto simp:
+      move12_def mem_empty_def mem_defs.map_of_def map_le_def update1_def update2_def Memory_Heap.lookup1_def Memory_Heap.lookup2_def get_k1_def get_k2_def mem_update_def Memory_Heap.mem_lookup_def
+      execute_bind_success[OF success_newI] execute_simps Let_def Array.get_alloc length_def
+      simp: inv_pair_presentD inv_pair_presentD2 
+      intro: alloc_present alloc_present'
+      split: if_split_asm
+    )
+    using injective
+    apply (subst (asm) nth_list_update_neq)
+    by auto
+  subgoal
+    apply (frule inv_pair_lengthD1)
+    apply (frule inv_pair_lengthD2)
+    apply (frule inv_pair_not_eqD)
+    apply (auto simp:
+      move12_def mem_empty_def mem_defs.map_of_def map_le_def update1_def update2_def Memory_Heap.lookup1_def Memory_Heap.lookup2_def get_k1_def get_k2_def mem_update_def Memory_Heap.mem_lookup_def
+      execute_bind_success[OF success_newI] execute_simps Let_def Array.get_alloc length_def
+      simp: inv_pair_presentD inv_pair_presentD2 
+      intro: alloc_present alloc_present'
+      split: if_split_asm
+      dest: Array.noteq_sym
+    )
+    done
+   subgoal for m k' v
+    apply (frule inv_pair_lengthD1)
+     apply (frule inv_pair_lengthD2)
+     apply (frule inv_pair_not_eqD)
+    apply (auto simp:
+      move12_def mem_empty_def mem_defs.map_of_def map_le_def update1_def update2_def Memory_Heap.lookup1_def Memory_Heap.lookup2_def get_k1_def get_k2_def mem_update_def Memory_Heap.mem_lookup_def
+      execute_bind_success[OF success_newI] execute_simps Let_def Array.get_alloc length_def
+      simp: inv_pair_presentD inv_pair_presentD2 
+      intro: alloc_present alloc_present'
+      split: if_split_asm
+    )
+     done
+   done
+
+ thm pair.lookup_pair_def pair.update_pair_def
+
+lemma state_of_bind:
+  "(state_of m1 \<bind> (\<lambda> x. state_of (m2 x))) = state_of (m1 \<bind> (\<lambda> x. m2 x))"
+  
+
+lemma
+  "runState (pair.update_pair k v) heap = runState (state_of (update_pair k v)) heap"
+  unfolding pair.update_pair_def update_pair_def
+  unfolding get_k1_def update1_def get_k2_def update2_def lookup1_def lookup2_def move12_def
+  apply simp
+
+lemma
+  "pair.update_pair k v = state_of (update_pair k v)"
+  unfolding pair.update_pair_def update_pair_def state_of_def
+  
+
+lemma mem_correct_pair:
+  "heap_correct inv_pair update_pair lookup_pair"
+proof (standard, goal_cases)
+  case (1 k) -- "Lookup invariant"
+  show ?case
+    unfolding lookup_pair_def Let_def State_Heap.lift_p_def
+    apply (auto intro!: lift_pI split: option.split simp: execute_simps)
+    using m1.lookup_inv m2.lookup_inv
+              apply (auto 7 2 dest: inv_pair_P_D1 inv_pair_P_D2 elim: lift_p_None[rotated 2])
+    unfolding inv_pair_def using injective
+    by (auto simp: execute_simps P_def Memory_Heap.mem_lookup_def Let_def split: if_split_asm)
+next
+  case (2 k v) -- "Update invariant"
+  show ?case
+    unfolding update_pair_def Let_def State_Heap.lift_p_def mem_empty_def
+    apply (auto intro!: lift_pI split: option.split simp: execute_simps)
+                        apply (auto intro!: lift_pI split: option.split prod.split_asm simp: execute_simps bind_def; fail)
+    using m1.update_inv m2.update_inv
+                        apply (auto 7 2 dest: inv_pair_P_D1 inv_pair_P_D2 elim: lift_p_None[rotated 2])
+using m1.update_inv m2.update_inv
+               apply (auto 9 2 dest: inv_pair_P_D1 inv_pair_P_D2 elim: lift_p_None[rotated 2])
+unfolding inv_pair_def using injective
+       apply (auto simp: execute_simps P_def Memory_Heap.mem_update_def Let_def split: if_split_asm; fail)+
+      defer
+      defer
+  defer
+unfolding inv_pair_def using injective
+      apply (auto simp: execute_simps P_def Memory_Heap.mem_update_def Let_def split: if_split_asm; fail)+
+
+    oops
+                   apply (auto intro!: lift_pI split: option.split prod.split_asm simp: execute_simps bind_def; fail)
+                  apply (auto intro!: lift_pI split: option.split prod.split_asm simp: execute_simps bind_def; fail)
+                 apply (auto intro!: lift_pI split: option.split prod.split_asm simp: execute_simps bind_def; fail)
+                apply (auto intro!: lift_pI split: option.split prod.split_asm simp: execute_simps bind_def; fail)
+apply (auto intro!: lift_pI split: option.split prod.split_asm simp: execute_simps bind_def; fail)
+    oops
+    using m1.lookup_inv m2.lookup_inv
+              apply (auto 7 2 dest: inv_pair_P_D1 inv_pair_P_D2 elim: lift_p_None[rotated 2])
+    unfolding inv_pair_def using injective
+    by (auto simp: execute_simps P_def Memory_Heap.mem_lookup_def Let_def split: if_split_asm)
+  with update_inv[of k v] update_correct[OF P_empty, of k v] P_empty show ?case
+    unfolding update_pair_def Let_def
+    by (auto intro!: lift_pI split: pair_storage.split_asm if_split_asm prod.split_asm)
+       (auto dest: lift_p_P simp: inv_pair_def,
+         (force dest: lift_p_P dest!: update_correct[of _ k v] map_le_implies_dom_le)+
+       )
+next
+  case (3 m k)
+  {
+    fix m1 v1 m1' m2 v2 m2' k1 k2
+    assume assms:
+      "runState (lookup k) m1 = (v1, m1')" "runState (lookup k) m2 = (v2, m2')"
+      "inv_pair (Pair_Storage k1 k2 m1 m2)"
+    from assms have "P m1" "P m2"
+      by (auto intro: inv_pair_P_D1 inv_pair_P_D2)
+    have [intro]: "map_of m1' \<subseteq>\<^sub>m map_of m1" "map_of m2' \<subseteq>\<^sub>m map_of m2"
+      using lookup_correct[OF \<open>P m1\<close>, of k] lookup_correct[OF \<open>P m2\<close>, of k] assms by auto
+    from inv_pair_domD[OF assms(3)] have 1: "dom (map_of m1') \<inter> dom (map_of m2) = {}"
+      by (metis (no_types) \<open>map_of m1' \<subseteq>\<^sub>m map_of m1\<close> disjoint_iff_not_equal domIff map_le_def)
+    have inv1: "inv_pair (Pair_Storage (key k) k2 m1' m2)" if "k2 \<noteq> key k" "k1 = key k"
+      using that \<open>P m1\<close> \<open>P m2\<close> unfolding inv_pair_def
+      apply clarsimp
+      apply safe
+      subgoal for x' y
+        using assms(1,3) lookup_correct[OF \<open>P m1\<close>, of k, THEN map_le_implies_dom_le]
+        unfolding inv_pair_def by auto
+      subgoal for x' y
+        using assms(3) unfolding inv_pair_def by fastforce
+      using lookup_inv[of k] assms unfolding lift_p_def by force
+    have inv2: "inv_pair (Pair_Storage k1 (key k) m1 m2')" if "k2 = key k" "k1 \<noteq> key k"
+      using that \<open>P m1\<close> \<open>P m2\<close> unfolding inv_pair_def
+      apply clarsimp
+      apply safe
+      subgoal for x' y
+        using assms(3) unfolding inv_pair_def by fastforce
+      subgoal for x x' y
+        using assms(2,3) lookup_correct[OF \<open>P m2\<close>, of k, THEN map_le_implies_dom_le]
+        unfolding inv_pair_def by fastforce
+      using lookup_inv[of k] assms unfolding lift_p_def by force
+    have A:
+      "pair.map_of (Pair_Storage (key k) k2 m1' m2) \<subseteq>\<^sub>m pair.map_of (Pair_Storage (key k) k2 m1 m2)"
+      if "k2 \<noteq> key k" "k1 = key k"
+      using inv1 assms(3) 1
+      by (auto intro: map_add_mono map_le_refl simp: that map_of_eq_pair[symmetric])
+    have B:
+      "pair.map_of (Pair_Storage k1 (key k) m1 m2') \<subseteq>\<^sub>m pair.map_of (Pair_Storage k1 (key k) m1 m2)"
+      if "k2 = key k" "k1 \<noteq> key k"
+      using inv2 assms(3) that
+      by (auto intro: map_add_mono map_le_refl simp: map_of_eq_pair[symmetric] dest: inv_pair_domD)
+    note A B
+  }
+  with \<open>inv_pair m\<close> show ?case
+    by (auto split: pair_storage.split if_split prod.split simp: Let_def lookup_pair_def)
+next
+  case (4 m k v)
+  {
+    fix m1 v1 m1' m2 v2 m2' m3 k1 k2
+    assume assms:
+      "runState (update k v) m1 = ((), m1')" "runState (update k v) m2 = ((), m2')"
+      "runState (update k v) empty = ((), m3)"
+      "inv_pair (Pair_Storage k1 k2 m1 m2)"
+    from assms have "P m1" "P m2"
+      by (auto intro: inv_pair_P_D1 inv_pair_P_D2)
+    from assms(3) P_empty update_inv[of k v] have "P m3"
+      unfolding lift_p_def by auto
+    have [intro]: "map_of m1' \<subseteq>\<^sub>m map_of m1(k \<mapsto> v)" "map_of m2' \<subseteq>\<^sub>m map_of m2(k \<mapsto> v)"
+      using update_correct[OF \<open>P m1\<close>, of k v] update_correct[OF \<open>P m2\<close>, of k v] assms by auto
+    have "map_of m3 \<subseteq>\<^sub>m map_of empty(k \<mapsto> v)"
+      using assms(3) update_correct[OF P_empty, of k v] by auto
+    also have "\<dots> \<subseteq>\<^sub>m map_of m2(k \<mapsto> v)"
+      using empty_correct by (auto elim: map_le_trans intro!: map_le_upd)
+    finally have "map_of m3 \<subseteq>\<^sub>m map_of m2(k \<mapsto> v)" .
+    have 1: "dom (map_of m1) \<inter> dom (map_of m2(k \<mapsto> v)) = {}" if "k1 \<noteq> key k"
+      using assms(4) that by (force simp: inv_pair_def)
+    have 2: "dom (map_of m3) \<inter> dom (map_of m1) = {}" if "k1 \<noteq> key k"
+      using \<open>local.map_of m3 \<subseteq>\<^sub>m local.map_of empty(k \<mapsto> v)\<close> assms(4) that
+      by (fastforce dest!: map_le_implies_dom_le simp: inv_pair_def)
+    have inv: "inv_pair (Pair_Storage (key k) k1 m3 m1)" if "k2 \<noteq> key k" "k1 \<noteq> key k"
+      using that \<open>P m1\<close> \<open>P m2\<close> \<open>P m3\<close> unfolding inv_pair_def
+      apply clarsimp
+      apply safe
+      subgoal for x x' y
+        using assms(3) update_correct[OF P_empty, of k v, THEN map_le_implies_dom_le]
+          empty_correct
+        by (auto dest: map_le_implies_dom_le)
+      subgoal for x x' y
+        using assms(4) unfolding inv_pair_def by fastforce
+      done
+    have A:
+      "pair.map_of (Pair_Storage (key k) k1 m3 m1) \<subseteq>\<^sub>m pair.map_of (Pair_Storage k1 k2 m1 m2)(k \<mapsto> v)"
+      if "k2 \<noteq> key k" "k1 \<noteq> key k"
+      using inv assms(4) \<open>map_of m3 \<subseteq>\<^sub>m map_of m2(k \<mapsto> v)\<close> 1
+      apply (simp add: that map_of_eq_pair[symmetric])
+      apply (subst map_add_upd[symmetric], subst Map.map_add_comm, rule 2, rule that)
+      by (rule map_add_mono; auto)
+    have inv1: "inv_pair (Pair_Storage (key k) k2 m1' m2)" if "k2 \<noteq> key k" "k1 = key k"
+      using that \<open>P m1\<close> \<open>P m2\<close> unfolding inv_pair_def
+      apply clarsimp
+      apply safe
+      subgoal for x' y
+        using assms(1,4) update_correct[OF \<open>P m1\<close>, of k v, THEN map_le_implies_dom_le]
+        unfolding inv_pair_def by auto
+      subgoal for x' y
+        using assms(4) unfolding inv_pair_def by fastforce
+      using update_inv[of k v] assms unfolding lift_p_def by force
+    have inv2: "inv_pair (Pair_Storage k1 (key k) m1 m2')" if "k2 = key k" "k1 \<noteq> key k"
+      using that \<open>P m1\<close> \<open>P m2\<close> unfolding inv_pair_def
+      apply clarsimp
+      apply safe
+      subgoal for x' y
+        using assms(4) unfolding inv_pair_def by fastforce
+      subgoal for x x' y
+        using assms(2,4) update_correct[OF \<open>P m2\<close>, of k v, THEN map_le_implies_dom_le]
+        unfolding inv_pair_def by fastforce
+      using update_inv[of k v] assms unfolding lift_p_def by force
+    have C:
+      "pair.map_of (Pair_Storage (key k) k2 m1' m2) \<subseteq>\<^sub>m
+       pair.map_of (Pair_Storage (key k) k2 m1 m2)(k \<mapsto> v)"
+      if "k2 \<noteq> key k" "k1 = key k"
+      using inv1[OF that] assms(4) \<open>inv_pair m\<close>
+      by (simp add: that map_of_eq_pair[symmetric])
+         (subst map_add_upd2[symmetric]; force simp: inv_pair_def intro: map_add_mono map_le_refl)
+    have B:
+      "pair.map_of (Pair_Storage k1 (key k) m1 m2') \<subseteq>\<^sub>m
+       pair.map_of (Pair_Storage k1 (key k) m1 m2)(k \<mapsto> v)"
+      if "k2 = key k" "k1 \<noteq> key k"
+      using inv2[OF that] assms(4)
+      by (simp add: that map_of_eq_pair[symmetric])
+         (subst map_add_upd[symmetric]; rule map_add_mono; force simp: inv_pair_def)
+    note A B C
+  }
+  with \<open>inv_pair m\<close> show ?case
+    by (auto split: pair_storage.split if_split prod.split simp: Let_def update_pair_def)
+qed
+
+definition
+  "inv_pair heap = (
+    let
+      k1 = Ref.get heap k_ref1;
+      k2 = Ref.get heap k_ref2;
+      m1 = Ref.get heap m_ref1;
+      m2 = Ref.get heap m_ref2
+    in
+      key1 ` dom (heap_mem_defs.map_of_heap (mem_lookup m1) heap) \<subseteq> {k1} \<and>
+      key1 ` dom (heap_mem_defs.map_of_heap (mem_lookup m2) heap) \<subseteq> {k2} \<and>
+      k1 \<noteq> k2
+  )"
+
+definition
+  "inv_pair = (!k_ref1 \<bind> (\<lambda> k1. !k_ref2 \<bind> (\<lambda> k2. !m_ref1 \<bind> (\<lambda> m1. !m_ref2 \<bind> (\<lambda> m2.
+    True
+    ))))
+  )"
+
+end
+
 end (* Injectivity *)
+
+locale heap_mem_empty_defs =
+  heap_mem_defs P lookup update for P and lookup and update :: "'k \<Rightarrow> 'v \<Rightarrow> unit Heap" +
+  fixes empty :: ""
+begin
 
 end (* Theory *)
