scratch/Memory.thy
@@ -37,6 +37,397 @@ lemma map_add_upd2:
   using that
   by auto
 
+
+(*
+locale mem_correct_empty = mem_correct +
+  fixes empty
+  assumes empty_correct: "map_of empty \<subseteq>\<^sub>m Map.empty" and P_empty: "P empty"
+
+context mem_correct_empty
+begin
+*)
+
+locale pair_mem_defs =
+  fixes lookup1 lookup2 :: "'a =='mem \<Longrightarrow> 'v option"
+    and update1 update2 :: "'a \<Rightarrow> 'v =='mem \<Longrightarrow> unit"
+    and move12 :: "'k1 \<Rightarrow> ('mem, unit) state"
+    and get_k1 get_k2 :: "('mem, 'k1) state"
+    and P :: "'mem \<Rightarrow> bool"
+  fixes key1 :: "'k \<Rightarrow> 'k1" and key2 :: "'k \<Rightarrow> 'a"
+begin
+
+text \<open>We assume that look-ups happen on the older row, so it is biased towards the second entry.\<close>
+definition
+  "lookup_pair k = do {
+     let k' = key1 k;
+     k2 \<leftarrow> get_k2;
+     if k' = k2
+     then lookup2 (key2 k)
+     else do {
+       k1 \<leftarrow> get_k1;
+       if k' = k1
+       then lookup1 (key2 k)
+       else return None
+     }
+   }
+   "
+
+text \<open>We assume that updates happen on the newer row, so it is biased towards the first entry.\<close>
+definition
+  "update_pair k v = do {
+    let k' = key1 k;
+    k1 \<leftarrow> get_k1;
+    if k' = k1
+    then update1 (key2 k) v
+    else do {
+      k2 \<leftarrow> get_k2;
+      if k' = k2
+      then update2 (key2 k) v
+      else (move12 k' \<then> update1 (key2 k) v)
+    }
+  }
+  "
+
+sublocale pair: mem_defs lookup_pair update_pair .
+
+sublocale mem1: mem_defs lookup1 update1 .
+
+sublocale mem2: mem_defs lookup2 update2 .
+
+definition
+  "inv_pair heap \<equiv>
+    let
+      k1 = fst (runState get_k1 heap);
+      k2 = fst (runState get_k2 heap)
+    in
+    (\<forall> k \<in> dom (mem1.map_of heap). \<exists> k'. key1 k' = k1 \<and> key2 k' = k) \<and>
+    (\<forall> k \<in> dom (mem2.map_of heap). \<exists> k'. key1 k' = k2 \<and> key2 k' = k) \<and>
+    k1 \<noteq> k2 \<and> P heap
+  "
+
+definition
+  "map_of1 m k = (if key1 k = fst (runState get_k1 m) then mem1.map_of m (key2 k) else None)"
+
+definition
+  "map_of2 m k = (if key1 k = fst (runState get_k2 m) then mem2.map_of m (key2 k) else None)"
+
+end (* Pair Mem Defs *)
+
+locale pair_mem = pair_mem_defs +
+  assumes get_state:
+    "runState get_k1 m = (k, m') \<Longrightarrow> m' = m"
+    "runState get_k2 m = (k, m') \<Longrightarrow> m' = m"
+  assumes move12_correct:
+    "P m \<Longrightarrow> runState (move12 k1) m = (x, m') \<Longrightarrow> mem1.map_of m' \<subseteq>\<^sub>m Map.empty"
+    "P m \<Longrightarrow> runState (move12 k1) m = (x, m') \<Longrightarrow> mem2.map_of m' \<subseteq>\<^sub>m mem1.map_of m"
+  assumes move12_keys:
+    "runState (move12 k1) m = (x, m') \<Longrightarrow> fst (runState get_k1 m') = k1"
+    "runState (move12 k1) m = (x, m') \<Longrightarrow> fst (runState get_k2 m') = fst (runState get_k1 m)"
+  assumes move12_inv:
+    "lift_p P (move12 k1)"
+  assumes lookup_inv:
+    "lift_p P (lookup1 k')" "lift_p P (lookup2 k')"
+  assumes update_inv:
+    "lift_p P (update1 k' v)" "lift_p P (update2 k' v)"
+  assumes lookup_keys:
+    "P m \<Longrightarrow> runState (lookup1 k') m = (v', m') \<Longrightarrow>
+     fst (runState get_k1 m') = fst (runState get_k1 m)"
+    "P m \<Longrightarrow> runState (lookup1 k') m = (v', m') \<Longrightarrow>
+     fst (runState get_k2 m') = fst (runState get_k2 m)"
+    "P m \<Longrightarrow> runState (lookup2 k') m = (v', m') \<Longrightarrow>
+     fst (runState get_k1 m') = fst (runState get_k1 m)"
+    "P m \<Longrightarrow> runState (lookup2 k') m = (v', m') \<Longrightarrow>
+     fst (runState get_k2 m') = fst (runState get_k2 m)"
+  assumes update_keys:
+    "P m \<Longrightarrow> runState (update1 k' v) m = (x, m') \<Longrightarrow>
+     fst (runState get_k1 m') = fst (runState get_k1 m)"
+    "P m \<Longrightarrow> runState (update1 k' v) m = (x, m') \<Longrightarrow>
+     fst (runState get_k2 m') = fst (runState get_k2 m)"
+    "P m \<Longrightarrow> runState (update2 k' v) m = (x, m') \<Longrightarrow>
+     fst (runState get_k1 m') = fst (runState get_k1 m)"
+    "P m \<Longrightarrow> runState (update2 k' v) m = (x, m') \<Longrightarrow>
+     fst (runState get_k2 m') = fst (runState get_k2 m)"
+  assumes
+    lookup_correct:
+      "P m \<Longrightarrow> mem1.map_of (snd (runState (lookup1 k') m)) \<subseteq>\<^sub>m (mem1.map_of m)"
+      "P m \<Longrightarrow> mem2.map_of (snd (runState (lookup1 k') m)) \<subseteq>\<^sub>m (mem2.map_of m)"
+      "P m \<Longrightarrow> mem1.map_of (snd (runState (lookup2 k') m)) \<subseteq>\<^sub>m (mem1.map_of m)"
+      "P m \<Longrightarrow> mem2.map_of (snd (runState (lookup2 k') m)) \<subseteq>\<^sub>m (mem2.map_of m)"
+  assumes
+    update_correct:
+      "P m \<Longrightarrow> mem1.map_of (snd (runState (update1 k' v) m)) \<subseteq>\<^sub>m (mem1.map_of m)(k' \<mapsto> v)"
+      "P m \<Longrightarrow> mem2.map_of (snd (runState (update2 k' v) m)) \<subseteq>\<^sub>m (mem2.map_of m)(k' \<mapsto> v)"
+      "P m \<Longrightarrow> mem2.map_of (snd (runState (update1 k' v) m)) \<subseteq>\<^sub>m mem2.map_of m"
+      "P m \<Longrightarrow> mem1.map_of (snd (runState (update2 k' v) m)) \<subseteq>\<^sub>m mem1.map_of m"
+begin
+
+lemma map_of_le_pair:
+  "pair.map_of m \<subseteq>\<^sub>m map_of1 m ++ map_of2 m"
+  if "inv_pair m"
+  using that
+  unfolding pair.map_of_def map_of1_def map_of2_def
+  unfolding lookup_pair_def inv_pair_def map_of_def map_le_def dom_def map_add_def
+  unfolding bind_def
+  by (auto 4 4
+        simp: mem2.map_of_def mem1.map_of_def runState_return Let_def
+        dest: get_state split: prod.split_asm if_split_asm
+     )
+
+lemma pair_le_map_of:
+  "map_of1 m ++ map_of2 m \<subseteq>\<^sub>m pair.map_of m"
+  if "inv_pair m"
+  using that
+  unfolding pair.map_of_def map_of1_def map_of2_def
+  unfolding lookup_pair_def inv_pair_def map_of_def map_le_def dom_def map_add_def
+  unfolding bind_def
+  by (auto
+        simp: mem2.map_of_def mem1.map_of_def runState_return Let_def
+        dest: get_state split: prod.splits if_split_asm option.split
+     )
+
+lemma map_of_eq_pair:
+  "map_of1 m ++ map_of2 m = pair.map_of m"
+  if "inv_pair m"
+  using that
+  unfolding pair.map_of_def map_of1_def map_of2_def
+  unfolding lookup_pair_def inv_pair_def map_of_def map_le_def dom_def map_add_def
+  unfolding bind_def
+  by (auto 4 4
+        simp: mem2.map_of_def mem1.map_of_def runState_return Let_def
+        dest: get_state split: prod.splits option.split
+     )
+
+lemma inv_pair_neq[simp]:
+  False if "inv_pair m" "fst (runState get_k1 m) = fst (runState get_k2 m)"
+  using that unfolding inv_pair_def by auto
+
+lemma inv_pair_P_D:
+  "P m" if "inv_pair m"
+  using that unfolding inv_pair_def by (auto simp: Let_def)
+
+lemma inv_pair_domD[intro]:
+  "dom (map_of1 m) \<inter> dom (map_of2 m) = {}" if "inv_pair m"
+  using that unfolding inv_pair_def map_of1_def map_of2_def by (auto split: if_split_asm)
+
+lemma move12_correct1:
+  "map_of1 heap' \<subseteq>\<^sub>m Map.empty" if "runState (move12 k1) heap = (x, heap')" "P heap"
+  using move12_correct[OF that(2,1)] unfolding map_of1_def by (auto simp: move12_keys map_le_def)
+
+lemma move12_correct2:
+  "map_of2 heap' \<subseteq>\<^sub>m map_of1 heap" if "runState (move12 k1) heap = (x, heap')" "P heap"
+  using move12_correct(2)[OF that(2,1)] that unfolding map_of1_def map_of2_def
+  by (auto simp: move12_keys map_le_def)
+
+lemma dom_empty[simp]:
+  "dom (map_of1 heap') = {}" if "runState (move12 k1) heap = (x, heap')" "P heap"
+  using move12_correct1[OF that] by (auto dest: map_le_implies_dom_le)
+
+lemma inv_pair_lookup1:
+  "inv_pair m'" if "runState (lookup1 k) m = (v, m')" "inv_pair m"
+  using that lookup_inv[of k] inv_pair_P_D[OF \<open>inv_pair m\<close>] unfolding inv_pair_def
+  by (auto 4 4
+        simp: Let_def lookup_keys
+        dest: lift_p_P lookup_correct[of _ k, THEN map_le_implies_dom_le]
+     )
+
+lemma inv_pair_lookup2:
+  "inv_pair m'" if "runState (lookup2 k) m = (v, m')" "inv_pair m"
+  using that lookup_inv[of k] inv_pair_P_D[OF \<open>inv_pair m\<close>] unfolding inv_pair_def
+  by (auto 4 4
+        simp: Let_def lookup_keys
+        dest: lift_p_P lookup_correct[of _ k, THEN map_le_implies_dom_le]
+     )
+
+lemma inv_pair_update1:
+  "inv_pair m'"
+  if "runState (update1 (key2 k) v) m = (v', m')" "inv_pair m" "fst (runState get_k1 m) = key1 k"
+  using that update_inv[of "key2 k" v] inv_pair_P_D[OF \<open>inv_pair m\<close>] unfolding inv_pair_def
+  apply (auto
+        simp: Let_def update_keys
+        dest: lift_p_P update_correct[of _ "key2 k" v, THEN map_le_implies_dom_le]
+     )
+   apply (frule update_correct[of _ "key2 k" v, THEN map_le_implies_dom_le]; auto 13 2; fail)
+  apply (frule update_correct[of _ "key2 k" v, THEN map_le_implies_dom_le]; auto 13 2; fail)
+  done
+
+lemma inv_pair_update2:
+  "inv_pair m'"
+  if "runState (update2 (key2 k) v) m = (v', m')" "inv_pair m" "fst (runState get_k2 m) = key1 k"
+  using that update_inv[of "key2 k" v] inv_pair_P_D[OF \<open>inv_pair m\<close>] unfolding inv_pair_def
+  apply (auto
+        simp: Let_def update_keys
+        dest: lift_p_P update_correct[of _ "key2 k" v, THEN map_le_implies_dom_le]
+     )
+   apply (frule update_correct[of _ "key2 k" v, THEN map_le_implies_dom_le]; auto 13 2; fail)
+  apply (frule update_correct[of _ "key2 k" v, THEN map_le_implies_dom_le]; auto 13 2; fail)
+  done
+
+lemma inv_pair_move12:
+  "inv_pair m'"
+  if "runState (move12 (key1 k)) m = (v', m')" "inv_pair m" "fst (runState get_k1 m) \<noteq> key1 k"
+  using that move12_inv[of "key1 k"] inv_pair_P_D[OF \<open>inv_pair m\<close>] unfolding inv_pair_def
+  apply (auto
+        simp: Let_def move12_keys
+        dest: lift_p_P move12_correct[of _ "key1 k", THEN map_le_implies_dom_le]
+     )
+  apply (blast dest: move12_correct[of _ "key1 k", THEN map_le_implies_dom_le])
+  done
+
+lemma mem_correct_pair:
+  "mem_correct lookup_pair update_pair inv_pair"
+  if injective: "\<forall> k k'. key1 k = key1 k' \<and> key2 k = key2 k' \<longrightarrow> k = k'"
+proof (standard, goal_cases)
+  case (1 k) -- "Lookup invariant"
+  show ?case
+    unfolding lookup_pair_def Let_def
+    by (auto 4 4
+        intro!: lift_pI split: pair_storage.split_asm if_split_asm prod.split_asm
+        simp: bind_def runState_return dest: get_state inv_pair_lookup1 inv_pair_lookup2
+        )
+next
+  case (2 k v) -- "Update invariant"
+  show ?case
+    unfolding update_pair_def Let_def
+    apply (auto 4 4
+        intro!: lift_pI split: pair_storage.split_asm if_split_asm prod.split_asm
+        simp: bind_def get_state runState_return dest: get_state intro: inv_pair_update1 inv_pair_update2
+        )+
+    apply (rule inv_pair_update1, assumption)
+     apply (rule inv_pair_move12, assumption)
+      apply (auto dest: get_state; fail)
+     apply (subst get_state, assumption)
+     apply (subst get_state, assumption)
+    by (auto intro: move12_keys)
+next
+  case (3 m k)
+  {
+    have "pair.map_of (snd (runState (lookup2 (key2 k)) m)) \<subseteq>\<^sub>m pair.map_of m"
+      apply (subst map_of_eq_pair[symmetric])
+       defer
+       apply (subst map_of_eq_pair[symmetric])
+        apply (rule 3)
+       apply (rule map_add_mono)
+      subgoal
+        by (smt 3 domD domI inv_pair_P_D local.lookup_keys lookup_correct map_le_def map_of1_def surjective_pairing)
+      subgoal
+        by (smt 3 domD domI inv_pair_P_D local.lookup_keys(4) lookup_correct(4) map_le_def map_of2_def surjective_pairing)
+      subgoal
+        using 3 \<open>map_of1 (snd (runState (lookup2 (key2 k)) m)) \<subseteq>\<^sub>m map_of1 m\<close> inv_pair_domD map_le_implies_dom_le by fastforce
+      subgoal
+        using 3 inv_pair_lookup2 surjective_pairing by blast
+      done
+  }
+  moreover
+  { have "pair.map_of (snd (runState (lookup1 (key2 k)) m)) \<subseteq>\<^sub>m pair.map_of m"
+      apply (subst map_of_eq_pair[symmetric])
+       defer
+       apply (subst map_of_eq_pair[symmetric])
+        apply (rule 3)
+       apply (rule map_add_mono)
+      subgoal
+        by (smt 3 domD domI inv_pair_P_D lookup_keys lookup_correct map_le_def map_of1_def map_of2_def surjective_pairing)
+        apply (smt 3 domD domI inv_pair_P_D lookup_keys lookup_correct map_le_def map_of1_def map_of2_def surjective_pairing)
+      subgoal
+        using 3 \<open>map_of1 (snd (runState (lookup1 (key2 k)) m)) \<subseteq>\<^sub>m map_of1 m\<close> inv_pair_domD map_le_implies_dom_le by fastforce
+      subgoal
+        using 3 inv_pair_lookup1 surjective_pairing by blast
+      done
+  }
+  ultimately show ?case
+    by (auto
+        split:if_split prod.split
+        simp: Let_def lookup_pair_def bind_def runState_return dest: get_state intro: map_le_refl
+        )
+next
+  case prems: (4 m k v)
+  show ?case
+    apply (auto split: pair_storage.split if_split prod.split simp: Let_def update_pair_def bind_def runState_return dest: get_state intro: map_le_refl)
+  proof goal_cases
+    case (1 x2)
+    then show ?case
+      apply (subst map_of_eq_pair[symmetric])
+       defer
+       apply (subst map_of_eq_pair[symmetric])
+        apply (rule prems)
+       apply (subst map_add_upd2[symmetric])
+         prefer 3
+         apply (rule map_add_mono)
+      subgoal
+        by (smt domIff fst_conv fun_upd_apply get_state(1) injective inv_pair_P_D map_le_def pair_mem_defs.map_of1_def prems surjective_pairing update_correct(1) update_keys(1))
+      subgoal
+        by (smt domIff get_state(1) inv_pair_P_D map_le_def pair_mem_defs.map_of2_def prems surjective_pairing update_correct(3) update_keys(2))
+      subgoal
+        by (smt inv_pair_P_D[OF \<open>inv_pair m\<close>] Int_emptyI domIff eq_snd_iff get_state(1) inv_pair_neq map_of2_def pair_mem_defs.map_of1_def prems update_keys(1))
+      subgoal
+        by (simp add: inv_pair_domD prems)
+      subgoal
+        using inv_pair_neq map_of2_def prems by fastforce
+      subgoal
+        by (metis fst_conv get_state(1) inv_pair_update1 prems surjective_pairing)
+      done
+  next
+    case (2 x1 x2 x2a)
+    then show ?case
+      apply (subst map_of_eq_pair[symmetric])
+       defer
+       apply (subst map_of_eq_pair[symmetric])
+        apply (rule prems)
+       apply (subst map_add_upd[symmetric])
+       apply (rule map_add_mono)
+      subgoal
+        by (smt domIff fst_conv fun_upd_apply get_state injective inv_pair_P_D map_le_def pair_mem_defs.map_of1_def prems surjective_pairing update_correct update_keys)
+      subgoal
+        by (smt domD domI fst_conv get_state(1) get_state(2) injective inv_pair_P_D map_le_def map_upd_Some_unfold pair_mem_defs.map_of2_def prems surjective_pairing update_correct(2) update_keys(4))
+      subgoal
+        by (smt \<open>\<lbrakk>key1 k \<noteq> x1; runState get_k2 x2 = (key1 k, x2a); runState get_k1 m = (x1, x2)\<rbrakk> \<Longrightarrow> map_of1 (snd (runState (update2 (key2 k) v) x2a)) \<subseteq>\<^sub>m map_of1 m\<close> disjoint_iff_not_equal domIff fst_conv fun_upd_apply get_state(1) map_le_def map_of1_def pair_mem_defs.map_of2_def)
+      subgoal
+        by (metis fst_conv get_state inv_pair_update2 prems surjective_pairing)
+      done
+
+  next
+    case (3 x1 x2 x1a x2a x2b)
+    then show ?case
+      apply (subst map_of_eq_pair[symmetric])
+       defer
+       apply (subst map_of_eq_pair[symmetric])
+        apply (rule prems)
+       apply (subst (2) map_add_comm)
+        defer
+        apply (subst map_add_upd2[symmetric])
+          prefer 3
+          apply (rule map_add_mono)
+      subgoal
+        by (smt domIff fst_conv fun_upd_apply get_state(1) get_state(2) injective inv_pair_P_D inv_pair_move12 map_le_def move12_correct(1) move12_keys(1) pair_mem_defs.map_of1_def prems surjective_pairing update_correct(1) update_keys(1))
+      subgoal
+        apply (frule get_state)
+        apply (frule get_state(2))
+        apply simp
+        apply (frule map_le_trans[OF update_correct(3) move12_correct(2), of _ m "key1 k" _ "key2 k" v, rotated 2])
+        using inv_pair_P_D[OF prems] apply (erule lift_p_P[OF move12_inv])
+         apply (rule inv_pair_P_D[OF prems])
+        subgoal
+          unfolding map_le_def map_of2_def
+          apply auto
+          apply (frule move12_keys(2), simp)
+          by (metis domI inv_pair_def inv_pair_move12 map_of1_def move12_keys(2) prems surjective_pairing update_keys(2))
+        done
+      subgoal
+        by (smt disjoint_iff_not_equal domIff fst_conv get_state(1) get_state(2) inv_pair_P_D inv_pair_move12 move12_keys(1) pair_mem_defs.map_of1_def prems surjective_pairing update_keys(1))
+      subgoal
+        using inv_pair_domD[OF prems] by blast
+      subgoal
+        by (simp add: domIff map_of1_def)
+      subgoal
+        by (smt fst_conv get_state(1) get_state(2) inv_pair_move12 inv_pair_update1 move12_keys(1) prems surjective_pairing)
+      subgoal
+        by (simp add: inv_pair_domD prems)
+      done
+  qed
+qed
+
+end (* Pair Mem *)
+
+
 locale mem_correct_empty = mem_correct +
   fixes empty
   assumes empty_correct: "map_of empty \<subseteq>\<^sub>m Map.empty" and P_empty: "P empty"
@@ -86,9 +477,10 @@ definition
     k1 \<noteq> k2 \<and> P m1 \<and> P m2
   )"
 
-term "pair.map_of (Pair_Storage k1 k2 m1 m2)"
-
-term "\<lambda> k. if key1 k = k1 then map_of m1 (key2 k) else None"
+definition
+  "inv_pair_weak p = (case p of Pair_Storage k1 k2 m1 m2 \<Rightarrow>
+    P m1 \<and> P m2
+  )"
 
 definition
   "map_of' m k1 k = (if key1 k = k1 then map_of m (key2 k) else None)"
@@ -141,6 +533,89 @@ lemma dom_empty[simp]:
 lemma dom_unequal_keys:
   "dom (map_of' m1 k1) \<inter> dom (map_of' m2 k2) = {}" if "k1 \<noteq> k2"
   using that unfolding map_of'_def by (auto split: if_split_asm)
+
+definition
+  "lookup1 k \<equiv> State (\<lambda> mem.
+    case mem of Pair_Storage k1 k2 m1 m2 \<Rightarrow>
+      case runState (lookup k) m1 of (v, m) \<Rightarrow> (v, Pair_Storage k1 k2 m m2))"
+
+definition
+  "lookup2 k \<equiv> State (\<lambda> mem.
+    case mem of Pair_Storage k1 k2 m1 m2 \<Rightarrow>
+      case runState (lookup k) m2 of (v, m) \<Rightarrow> (v, Pair_Storage k1 k2 m1 m))"
+
+definition
+  "update1 k v \<equiv> State (\<lambda> mem.
+    case mem of Pair_Storage k1 k2 m1 m2 \<Rightarrow>
+      case runState (update k v) m1 of (_, m) \<Rightarrow> ((), Pair_Storage k1 k2 m m2))"
+
+definition
+  "update2 k v \<equiv> State (\<lambda> mem.
+    case mem of Pair_Storage k1 k2 m1 m2 \<Rightarrow>
+      case runState (update k v) m2 of (_, m) \<Rightarrow> ((), Pair_Storage k1 k2 m1 m))"
+
+definition
+  "move12 k \<equiv> State (\<lambda> mem. case mem of Pair_Storage k1 k2 m1 m2 \<Rightarrow> ((), Pair_Storage k k1 empty m1))"
+
+definition
+  "get_k1 \<equiv> State (\<lambda> mem. case mem of Pair_Storage k1 k2 m1 m2 \<Rightarrow> (k1, mem))"
+
+definition
+  "get_k2 \<equiv> State (\<lambda> mem. case mem of Pair_Storage k1 k2 m1 m2 \<Rightarrow> (k2, mem))"
+
+lemma map_of_lookup1[simp]:
+  "mem_defs.map_of lookup1 (Pair_Storage k1 k2 m1 m2) = map_of m1"
+  unfolding mem_defs.map_of_def lookup1_def by (auto split: prod.split)
+
+lemma map_of_lookup2[simp]:
+  "mem_defs.map_of lookup2 (Pair_Storage k1 k2 m1 m2) = map_of m2"
+  unfolding mem_defs.map_of_def lookup2_def by (auto split: prod.split)
+
+lemma inv_pair_weakD1:
+  "P m1" if "inv_pair_weak (Pair_Storage k1 k2 m1 m2)"
+  using that unfolding inv_pair_weak_def by auto
+
+lemma inv_pair_weakD2:
+  "P m2" if "inv_pair_weak (Pair_Storage k1 k2 m1 m2)"
+  using that unfolding inv_pair_weak_def by auto
+
+lemma lookup_correct':
+  "P m \<Longrightarrow> runState (lookup k) m = (v, m') \<Longrightarrow> map_of m' \<subseteq>\<^sub>m (map_of m)"
+  using lookup_correct[of m k] by auto
+
+lemma update_correct':
+  "P m \<Longrightarrow> runState (update k v) m = (v', m') \<Longrightarrow> map_of m' \<subseteq>\<^sub>m (map_of m)(k \<mapsto> v)"
+  using update_correct[of m k v] by auto
+
+lemma pair_mem: "pair_mem lookup1 lookup2 update1 update2 move12 get_k1 get_k2 inv_pair_weak"
+  apply standard
+                      apply (auto split: pair_storage.splits simp: empty_correct get_k1_def get_k2_def move12_def; fail)+
+                      apply (auto intro!: lift_pI simp: inv_pair_weak_def move12_def P_empty lookup1_def lookup2_def update1_def update2_def split: pair_storage.splits prod.split_asm elim: lift_p_P[OF lookup_inv] lift_p_P[OF update_inv]; fail)+
+                 apply (auto split: pair_storage.split prod.split_asm simp: update1_def update2_def lookup1_def lookup2_def get_k1_def get_k2_def; fail)+
+  by (auto elim: update_correct' lookup_correct' dest: inv_pair_weakD1 inv_pair_weakD2 split: pair_storage.split prod.split simp: update1_def update2_def lookup1_def lookup2_def; fail)+
+
+interpretation pair: pair_mem lookup1 lookup2 update1 update2 move12 get_k1 get_k2 inv_pair_weak
+  by (rule pair_mem)
+
+lemma lookup_pair_alt_def:
+  "lookup_pair = pair.lookup_pair"
+  unfolding pair.lookup_pair_def lookup_pair_def
+  by (intro ext)
+     (auto
+       split: pair_storage.split prod.split
+       simp: lookup1_def lookup2_def bind_def runState_return Let_def get_k1_def get_k2_def
+     )
+
+lemma update_pair_alt_def:
+  "update_pair = pair.update_pair"
+  unfolding pair.update_pair_def update_pair_def
+  by (intro ext)
+     (auto
+       split: pair_storage.split prod.split
+       simp:
+        move12_def lookup1_def lookup2_def update1_def update2_def bind_def runState_return
+        Let_def get_k1_def get_k2_def
+     )
 
 lemma mem_correct_pair:
   "mem_correct lookup_pair update_pair inv_pair"
